fix argument order in refinement

bedrock2/src/bedrock2/Refinement.v
@@ -12,32 +12,32 @@ Section WithParams.
   Context {locals: map.map String.string word}.
   Context {ext_spec: bedrock2.Semantics.ExtSpec}.
 
-  Definition refinement(c1 c2: cmd) := forall functions t m l post,
+  Definition refines(c2 c1: cmd) := forall functions t m l post,
       Semantics.exec.exec functions c1 t m l post ->
       Semantics.exec.exec functions c2 t m l post.
 
   Lemma refinement_while: forall test body1 body2,
-      refinement body1 body2 ->
-      refinement (cmd.while test body1) (cmd.while test body2).
+      refines body2 body1 ->
+      refines (cmd.while test body2) (cmd.while test body1).
   Proof.
-    unfold refinement. intros * R *.
+    unfold refines. intros * R *.
     remember (cmd.while test body1) as c1. intros. revert Heqc1.
     induction H; intros; subst; inversion Heqc1; subst.
     - eapply Semantics.exec.while_false; eassumption.
     - eapply Semantics.exec.while_true; try eassumption.
-      { unfold refinement in R.
+      { unfold refines in R.
         eapply R. eassumption. }
       intros.
       eapply H3; eauto.
   Qed.
 
   Lemma refinement_seq: forall c1 c2 c1' c2',
-      refinement c1 c1' ->
-      refinement c2 c2' ->
-      refinement (cmd.seq c1 c2) (cmd.seq c1' c2').
+      refines c1' c1 ->
+      refines c2' c2 ->
+      refines (cmd.seq c1' c2') (cmd.seq c1 c2).
   Proof.
     intros * R1 R2 functions t m l post H.
-    unfold refinement in *.
+    unfold refines in *.
     inversion H. subst. clear H.
     eapply Semantics.exec.seq.
     - eapply R1. eassumption.
